Revert "Add partially minimized bug"
This reverts commit a6710276acb9a6f84f94ff32001b45b001574ce7.

quotation/theories/ToPCUIC/Init/Typing.v
@@ -1,180 +1,169 @@
-(* -*- mode: coq; coq-prog-args: ("-emacs" "-q" "-w" "-deprecated-native-compiler-option" "-native-compiler" "no" "-R" "/github/workspace/metacoq/utils/theories" "MetaCoq.Utils" "-R" "/github/workspace/metacoq/common/theories" "MetaCoq.Common" "-R" "/github/workspace/metacoq/pcuic/theories" "MetaCoq.PCUIC" "-R" "/github/workspace/metacoq/template-coq/theories" "MetaCoq.Template" "-R" "/github/workspace/metacoq/template-pcuic/theories" "MetaCoq.TemplatePCUIC" "-R" "/github/workspace/metacoq/safechecker/theories" "MetaCoq.SafeChecker" "-R" "/github/workspace/metacoq/quotation/theories" "MetaCoq.Quotation" "-Q" "/github/workspace/cwd" "Top" "-Q" "/home/coq/.opam/4.13.1+flambda/lib/coq/user-contrib/Bignums" "Bignums" "-Q" "/home/coq/.opam/4.13.1+flambda/lib/coq/user-contrib/Equations" "Equations" "-Q" "/home/coq/.opam/4.13.1+flambda/lib/coq/user-contrib/Ltac2" "Ltac2" "-I" "/github/workspace/metacoq/template-coq" "-top" "MetaCoq.Quotation.ToPCUIC.Init.Typing") -*- *)
-(* File reduced by coq-bug-minimizer from original input, then from 1736 lines to 188 lines, then from 201 lines to 687 lines, then from 692 lines to 320 lines *)
-(* coqc version 8.16.1 compiled with OCaml 4.13.1
-   coqtop version 8.16.1
-   Modules that could not be inlined: MetaCoq.Quotation.ToPCUIC.Coq.Init
-   Expected coqc runtime on this file: 4.956 sec *)
-Axiom proof_admitted : False.
-Tactic Notation "admit" := abstract case proof_admitted.
-Module Export PCUICErrors.
-
-Require MetaCoq.Utils.utils.
-Import MetaCoq.Utils.utils.
-
-Require MetaCoq.PCUIC.utils.PCUICPretty.
-Import MetaCoq.PCUIC.PCUICAst.
-
-Inductive ConversionError :=
-| NotFoundConstants (c1 c2 : kername)
-
-| NotFoundConstant (c : kername)
-
-| LambdaNotConvertibleTypes
-    (Γ1 : context) (na : aname) (A1 t1 : term)
-    (Γ2 : context) (na' : aname) (A2 t2 : term)
-    (e : ConversionError)
-
-| LambdaNotConvertibleAnn
-    (Γ1 : context) (na : aname) (A1 t1 : term)
-    (Γ2 : context) (na' : aname) (A2 t2 : term)
-
-| ProdNotConvertibleDomains
-    (Γ1 : context) (na : aname) (A1 B1 : term)
-    (Γ2 : context) (na' : aname) (A2 B2 : term)
-    (e : ConversionError)
-
-| ProdNotConvertibleAnn
-    (Γ1 : context) (na : aname) (A1 B1 : term)
-    (Γ2 : context) (na' : aname) (A2 B2 : term)
-
-| ContextNotConvertibleAnn
-    (Γ : context) (decl : context_decl)
-    (Γ' : context) (decl' : context_decl)
-| ContextNotConvertibleType
-    (Γ : context) (decl : context_decl)
-    (Γ' : context) (decl' : context_decl)
-| ContextNotConvertibleBody
-    (Γ : context) (decl : context_decl)
-    (Γ' : context) (decl' : context_decl)
-| ContextNotConvertibleLength
-
-| CaseOnDifferentInd
-    (Γ1 : context)
-    (ci : case_info) (p : predicate term) (c : term) (brs : list (branch term))
-    (Γ2 : context)
-    (ci' : case_info) (p' : predicate term) (c' : term) (brs' : list (branch term))
-
-| CasePredParamsUnequalLength
-    (Γ1 : context)
-    (ci : case_info) (p : predicate term) (c : term) (brs : list (branch term))
-    (Γ2 : context)
-    (ci' : case_info) (p' : predicate term) (c' : term) (brs' : list (branch term))
-
-| CasePredUnequalUniverseInstances
-    (Γ1 : context)
-    (ci : case_info) (p : predicate term) (c : term) (brs : list (branch term))
-    (Γ2 : context)
-    (ci' : case_info) (p' : predicate term) (c' : term) (brs' : list (branch term))
-
-| DistinctStuckProj
-    (Γ : context) (p : projection) (c : term)
-    (Γ' : context) (p' : projection) (c' : term)
-
-| CannotUnfoldFix
-    (Γ : context) (mfix : mfixpoint term) (idx : nat)
-    (Γ' : context) (mfix' : mfixpoint term) (idx' : nat)
-
-| FixRargMismatch (idx : nat)
-    (Γ : context) (u : def term) (mfix1 mfix2 : mfixpoint term)
-    (Γ' : context) (v : def term) (mfix1' mfix2' : mfixpoint term)
-
-| FixMfixMismatch (idx : nat)
-    (Γ : context) (mfix : mfixpoint term)
-    (Γ' : context) (mfix' : mfixpoint term)
-
-| DistinctCoFix
-    (Γ : context) (mfix : mfixpoint term) (idx : nat)
-    (Γ' : context) (mfix' : mfixpoint term) (idx' : nat)
-
-| CoFixRargMismatch (idx : nat)
-    (Γ : context) (u : def term) (mfix1 mfix2 : mfixpoint term)
-    (Γ' : context) (v : def term) (mfix1' mfix2' : mfixpoint term)
-
-| CoFixMfixMismatch (idx : nat)
-    (Γ : context) (mfix : mfixpoint term)
-    (Γ' : context) (mfix' : mfixpoint term)
-
-| StackHeadError
-    (leq : conv_pb)
-    (Γ1 : context)
-    (t1 : term) (args1 : list term) (u1 : term) (l1 : list term)
-    (Γ2 : context)
-    (t2 : term) (u2 : term) (l2 : list term)
-    (e : ConversionError)
-
-| StackTailError (leq : conv_pb)
-    (Γ1 : context)
-    (t1 : term) (args1 : list term) (u1 : term) (l1 : list term)
-    (Γ2 : context)
-    (t2 : term) (u2 : term) (l2 : list term)
-    (e : ConversionError)
-
-| StackMismatch
-    (Γ1 : context) (t1 : term) (args1 l1 : list term)
-    (Γ2 : context) (t2 : term) (l2 : list term)
-
-| HeadMismatch
-    (leq : conv_pb)
-    (Γ1 : context) (t1 : term)
-    (Γ2 : context) (t2 : term).
-
-Inductive type_error :=
-| UnboundRel (n : nat)
-| UnboundVar (id : string)
-| UnboundEvar (ev : nat)
-| UndeclaredConstant (c : kername)
-| UndeclaredInductive (c : inductive)
-| UndeclaredConstructor (c : inductive) (i : nat)
-| NotCumulSmaller {abstract_structure} (le : bool)
-  (G : abstract_structure) (Γ : context) (t u t' u' : term) (e : ConversionError)
-| NotConvertible {abstract_structure}
-  (G : abstract_structure)
-  (Γ : context) (t u : term)
-| NotASort (t : term)
-| NotAProduct (t t' : term)
-| NotAnInductive (t : term)
-| NotAnArity (t : term)
-| IllFormedFix (m : mfixpoint term) (i : nat)
-| UnsatisfiedConstraints (c : ConstraintSet.t)
-| Msg (s : string).
-
-Inductive env_error :=
-| IllFormedDecl (e : string) (e : type_error)
-| AlreadyDeclared (id : string).
-
-End PCUICErrors.
-Require MetaCoq.PCUIC.PCUICParallelReductionConfluence.
-Require MetaCoq.Quotation.ToPCUIC.Coq.Init.
-Import MetaCoq.Utils.utils.
-Import MetaCoq.Common.MonadBasicAst.
-Import MetaCoq.PCUIC.utils.PCUICAstUtils.
-Import MetaCoq.PCUIC.PCUICMonadAst.
-Import MetaCoq.PCUIC.PCUICAst.
-Import MetaCoq.PCUIC.PCUICTyping.
-Import MetaCoq.PCUIC.Syntax.PCUICReflect.
-Import MetaCoq.TemplatePCUIC.PCUICTemplateMonad.
-Import MetaCoq.TemplatePCUIC.Loader.
-Export MetaCoq.Quotation.ToPCUIC.Init.
+From MetaCoq.Utils Require Export bytestring.
+From MetaCoq.Utils Require Import utils MCList.
+From MetaCoq.Common Require Import MonadBasicAst.
+From MetaCoq.PCUIC.utils Require Import PCUICAstUtils.
+From MetaCoq.PCUIC Require Import PCUICMonadAst PCUICAst PCUICTyping PCUICSpine PCUICArities PCUICSubstitution.
+From MetaCoq.PCUIC.Typing Require Import PCUICWeakeningTyp PCUICWeakeningConfigTyp PCUICWeakeningEnvTyp PCUICClosedTyp.
+From MetaCoq.PCUIC.Syntax Require Import PCUICLiftSubst PCUICClosed PCUICInduction PCUICReflect.
+From MetaCoq.TemplatePCUIC Require Import PCUICTemplateMonad Loader.
+From MetaCoq.SafeChecker Require Import PCUICErrors PCUICTypeChecker PCUICSafeChecker PCUICWfEnvImpl PCUICWfEnv.
+From MetaCoq.Quotation Require Export CommonUtils.
+From MetaCoq.Quotation.ToPCUIC Require Export Init.
+From MetaCoq.Quotation.ToPCUIC Require Coq.Init.
 Import (hints) MetaCoq.Quotation.ToPCUIC.Coq.Init.
+Require Import Equations.Prop.Classes.
+Require Import Coq.Lists.List.
+Export TemplateMonad.Common (export, local, global).
+Import ListNotations.
 Import MCMonadNotation.
 Import PCUICEnvironmentReflect.
+(*
+From MetaCoq.Template Require Import MonadBasicAst MonadAst All utils.
+From MetaCoq.Template Require Import Typing utils.bytestring TermEquality ReflectAst Ast Reflect.
+From MetaCoq.Lob.Template Require Export QuoteGround.Init.
+Export utils.bytestring.
+Require Import Coq.Lists.List.
+Import ListNotations.
+
+Local Set Primitive Projections.
+Local Open Scope bs.
+Import MCMonadNotation.
+ *)
 
 Local Set Universe Polymorphism.
 Local Unset Universe Minimization ToSet.
-
+Local Set Polymorphic Inductive Cumulativity.
+(*
+Module config.
+  Class typing_restriction
+    := { checker_flags_constraint : config.checker_flags -> bool
+       ; global_env_ext_constraint : global_env_ext -> bool }.
+  Definition and_typing_restriction (x y : typing_restriction) : typing_restriction
+    := {| checker_flags_constraint cf := x.(checker_flags_constraint) cf && y.(checker_flags_constraint) cf;
+         global_env_ext_constraint Σ := x.(global_env_ext_constraint) Σ && y.(global_env_ext_constraint) Σ |}.
+  Definition or_typing_restriction (x y : typing_restriction) : typing_restriction
+    := {| checker_flags_constraint cf := x.(checker_flags_constraint) cf && y.(checker_flags_constraint) cf;
+         global_env_ext_constraint Σ := x.(global_env_ext_constraint) Σ && y.(global_env_ext_constraint) Σ |}.
+  Module Export Notations.
+    Declare Scope typing_restriction_scope.
+    Delimit Scope typing_restriction_scope with typing_restriction.
+    Bind Scope typing_restriction_scope with typing_restriction.
+    Infix "&&" := and_typing_restriction : typing_restriction_scope.
+    Infix "||" := or_typing_restriction : typing_restriction_scope.
+  End Notations.
+End config.
+Export config.Notations.
+*)
+(* TODO: Right now, quotation / translation always claims constants are monomorphic; if there's eventually support for polymorphic quotation, we may want to not restrict typing to be monomorphic here *)
 Class quotation_of_well_typed {cf : config.checker_flags} (Σ : global_env) {T} (t : T) {qT : quotation_of T} {qt : quotation_of t} := typing_quoted_term_of : wf Σ -> (Σ, Monomorphic_ctx) ;;; [] |- qt : qT.
 Class ground_quotable_well_typed {cf : config.checker_flags} (Σ : global_env) T {qT : quotation_of T} {quoteT : ground_quotable T} := typing_quote_ground : forall t : T, quotation_of_well_typed Σ t.
 
+Definition typing_quoted_term_of_general
+  {cf : config.checker_flags} {Σ : global_env} {T} (t : T) {qT : quotation_of T} {qt : quotation_of t}
+  {qty : @quotation_of_well_typed cf Σ T t _ _}
+  {cf' : config.checker_flags} {Σ' : global_env} {Γ}
+  : @wf cf Σ -> @wf cf' Σ' -> (let _ := cf' in wf_local (Σ', Monomorphic_ctx) Γ) -> extends Σ Σ' -> config.impl cf cf' -> @typing cf' (Σ', Monomorphic_ctx) Γ qt qT.
+Proof.
+  intros wfΣ wfΣ' wfΓ Hext Hcf.
+  specialize (qty wfΣ).
+  replace Γ with ([],,,Γ) by now rewrite app_context_nil_l.
+  erewrite <- (@lift_closed _ _ qt), <- (@lift_closed _ _ qT).
+  { eapply weakening; rewrite ?app_context_nil_l; try eassumption.
+    eapply (@weakening_env cf' (Σ, _)); try eassumption.
+    all: try now eapply (@weakening_config_wf cf cf'); assumption.
+    eapply (@weakening_config cf cf'); assumption. }
+  all: change 0 with #|[]:context|.
+  all: try (eapply (@subject_closed cf (_, _)); eassumption).
+  all: try (eapply (@type_closed cf (_, _)); eassumption).
+Qed.
+
+Definition typing_quoted_term_of_general_empty_ctx
+  {cf : config.checker_flags} {Σ : global_env} {T} (t : T) {qT : quotation_of T} {qt : quotation_of t}
+  {qty : @quotation_of_well_typed cf Σ T t _ _}
+  {cf' : config.checker_flags} {Σ' : global_env}
+  : @wf cf Σ -> @wf cf' Σ' -> extends Σ Σ' -> config.impl cf cf' -> @typing cf' (Σ', Monomorphic_ctx) [] qt qT.
+Proof.
+  intros; eapply (@typing_quoted_term_of_general cf Σ T t qT qt qty cf' Σ'); tea.
+  constructor.
+Qed.
+
+(*
+Class quotation_of_well_typed {Pcf : config.typing_restriction} {T} (t : T) {qT : quotation_of T} {qt : quotation_of t} := typing_quoted_term_of : forall cf Σ Γ, config.checker_flags_constraint cf -> config.global_env_ext_constraint Σ -> wf Σ -> wf_local Σ Γ -> Σ ;;; Γ |- qt : qT.
+Class ground_quotable_well_typed {Pcf : config.typing_restriction} T {qT : quotation_of T} {quoteT : ground_quotable T} := typing_quote_ground : forall t : T, quotation_of_well_typed t.
+*)
+Class infer_quotation_of_well_typed (qt : term)
+  := { wt_cf : config.checker_flags
+     ; wt_Σ : global_env
+     ; wt_T : Type
+     ; wt_t : wt_T
+     ; wt_qT : quotation_of wt_T
+     ; wt_qt : quotation_of wt_t := qt
+     ; wt_q : @quotation_of_well_typed wt_cf wt_Σ wt_T wt_t _ _ }.
+Class infer_type_of (qt : term) := qtype_of : term.
+Ltac infer_type_of qt
+  := lazymatch (eval hnf in (_ : infer_quotation_of_well_typed qt)) with
+     | {| wt_qT := ?qT |} => exact qT
+     end.
+
 Inductive dynlist := dnil | dcons {T} (t : T) (tl : dynlist).
+Declare Scope dynlist_scope.
 Delimit Scope dynlist_scope with dynlist.
+Bind Scope dynlist_scope with dynlist.
+Infix "::" := dcons : dynlist_scope.
+Notation "[ ]" := dnil : dynlist_scope.
+Notation "[ x ]" := (dcons x dnil) : dynlist_scope.
 Notation "[ x ; y ; .. ; z ]" :=  (dcons x (dcons y .. (dcons z dnil) ..)) : dynlist_scope.
 
+(*
+Fixpoint quote_dynlist (d : dynlist) : TemplateMonad (list term)
+  := match d with
+     | dnil => ret []
+     | dcons _ t rest => qt <- tmQuote t;; qts <- quote_dynlist rest;; ret (qt :: qts)
+     end.
+
+Definition constraint_for_globals (globals : dynlist) : TemplateMonad (global_env_ext -> bool)
+  := qts <- quote_dynlist globals;;
+     inds <- monad_map (fun qt => match Init.head qt with
+                                  | tInd {| inductive_mind := mind |} _
+                                    => ind <- tmQuoteInductive mind;;
+                                       (*tmPrint ind;;*)
+                                       ret (mind, ind)
+                                  | _ => tmPrint ("ensure present not inductive"%bs, qt);; tmFail "ensure present not inductive"%bs
+                                  end) qts;;
+     ret (fun Σ : global_env_ext
+          => List.fold_right andb true (List.map (fun '(mind, ind) => lookup_env Σ.1 mind == Some (InductiveDecl ind)) inds)).
+ *)
+(* don't use [dynlist] inductive when quoting *)
 Definition erase_dynlist (globals : dynlist)
   := Eval cbv [dynlist_ind] in fun P n c => dynlist_ind (fun _ => P) n (fun T t _ r => c T t r) globals.
-Definition env_for_globals (globals : forall P : Prop, P -> (forall x : Type, x -> P -> P) -> P) : TemplateMonad global_env_ext.
-exact (qglobals <- tmQuoteRec globals;;
-     ret (PCUICProgram.global_env_ext_map_global_env_ext (fst (qglobals:PCUICProgram.pcuic_program)))).
-Defined.
+Definition env_for_globals (globals : forall P : Prop, P -> (forall x : Type, x -> P -> P) -> P) : TemplateMonad global_env_ext
+  := qglobals <- tmQuoteRec globals;;
+     ret (PCUICProgram.global_env_ext_map_global_env_ext (fst (qglobals:PCUICProgram.pcuic_program))).
+
+Notation ground_quotable_well_typed_using ls T
+  := (match ls%dynlist, T return _ with
+      | globals, T'
+        => ltac:(let T' := (eval cbv delta [T'] in T') in
+                 let globals := (eval cbv [erase_dynlist globals] in (erase_dynlist globals)) in
+                 run_template_program
+                   (env_for_globals globals)
+                   (fun Σ => refine (@ground_quotable_well_typed
+                                       _ Σ
+                                       T' _ _)))
+      end)
+       (only parsing).
+Notation quotation_of_well_typed_using ls t
+  := (match ls%dynlist, t return _ with
+      | globals, t'
+        => ltac:(let t' := (eval cbv delta [t'] in t') in
+                 let globals := (eval cbv [erase_dynlist globals] in (erase_dynlist globals)) in
+                 run_template_program
+                   (env_for_globals globals)
+                   (fun Σ => refine (@quotation_of_well_typed
+                                       _ Σ
+                                       _ t' _ _)))
+      end)
+       (only parsing).
 Notation typing_restriction_for_globals ls
   := (match ls%dynlist return _ with
       | globals
@@ -184,29 +173,722 @@ Notation typing_restriction_for_globals ls
                    (fun Σ => refine Σ))
       end)
        (only parsing).
-Definition evalStateT {S M T} {TM : Monad M} (p : StateT S M T) (st : S) : M T.
-exact ('(v, st) <- p st;;
-     ret v).
+
+
+Module Export Instances.
+  #[export] Existing Instance Build_infer_quotation_of_well_typed.
+  #[export] Hint Extern 0 (infer_quotation_of_well_typed ?qt)
+  => simple notypeclasses refine (@Build_infer_quotation_of_well_typed qt _ _ _ _ _ _);
+     [ .. | typeclasses eauto ]
+       : typeclass_instances.
+  #[export] Hint Extern 0 (infer_type_of ?qt) => infer_type_of qt : typeclass_instances.
+  (* #[export] *)
+  Coercion wt_q : infer_quotation_of_well_typed >-> quotation_of_well_typed.
+  (*#[export] Instance default_typing_restriction : config.typing_restriction | 1000
+    := {| config.checker_flags_constraint cf := true
+       ; config.global_env_ext_constraint Σ := true |}.*)
+  #[export] Existing Instance typing_quote_ground.
+End Instances.
+
+Definition lift_step
+  : forall (lift' : nat -> nat -> term -> term) (n k : nat) (t : term), term.
+Proof.
+  let v := (eval cbv delta [lift] in lift) in
+  let liftTy := lazymatch goal with |- ?T -> _ => T end in
+  run_template_program
+    (lift <- tmQuote v;;
+     qliftTy <- tmQuote liftTy;;
+     match lift with
+     | tFix [b] _
+       => tmUnquote
+            (tLambda
+               {| binder_name := nNamed "lift'"; binder_relevance := Relevant |}
+               qliftTy
+               b.(dbody))
+     | _ => tmPrint lift;; tmFail "bad lift body"
+     end)
+    (fun v => lazymatch v with
+              | {| my_projT2 := ?v |} => exact v
+              end).
 Defined.
+
+Definition prelift (lift : nat -> nat -> term -> term) (n k : nat) (t : term) : term
+  := if match n with 0 => true | _ => false end
+     then t
+     else lift n k t.
+Fixpoint lift' n k t {struct t} := lift_step (prelift lift') n k t.
+Definition lift_opt n k t := prelift lift' n k t.
+
+Lemma eq_prelift lift n k t
+  : lift n k t = PCUICAst.lift n k t
+    -> prelift lift n k t = PCUICAst.lift n k t.
+Proof.
+  destruct n; cbn; auto.
+  rewrite !lift0_id; reflexivity.
+Qed.
+
+Lemma eq_lift' n k t : lift' n k t = PCUICAst.lift n k t.
+Proof.
+  revert n k; induction t using term_forall_list_ind; intros; cbn -[prelift]; try reflexivity.
+  all: f_equal.
+  all: repeat first [ progress intros
+                    | reflexivity
+                    | solve [ eauto ]
+                    | rewrite eq_prelift
+                    | apply map_ext_in_iff
+                    | apply map_def_eq_spec
+                    | apply map_predicate_k_eq_spec
+                    | apply map_branch_k_eq_spec
+                    | progress cbv [shiftf] ].
+  all: repeat first [ progress hnf in *
+                    | solve [ eauto ]
+                    | progress rdest
+                    | progress sq
+                    | match goal with
+                      | [ H : All _ _ |- _ ] => pose proof (fun X H' => @All_In _ _ _ X H' H); clear H
+                      | [ H : forall X, In X ?v -> _ |- _ ]
+                        => exactly_once (idtac; multimatch goal with
+                                                | [ H' : In _ v |- _ ]
+                                                  => specialize (H _ H')
+                                                end)
+                      end ].
+Qed.
+
+Lemma eq_lift_opt n k t : lift_opt n k t = PCUICAst.lift n k t.
+Proof.
+  cbv [lift_opt]; rewrite eq_prelift; rewrite ?eq_lift'; reflexivity.
+Qed.
+
+Definition subst_step (lift' : nat -> nat -> term -> term)
+  : forall (subst' : list term -> nat -> term -> term) (s : list term) (k : nat) (u : term), term.
+Proof.
+  let v := (eval cbv delta [subst] in subst) in
+  let v := lazymatch (eval pattern (@PCUICAst.lift) in v) with
+           | ?f _ => f
+           end in
+  let v := (eval cbv beta in (v lift')) in
+  let substTy := lazymatch goal with |- ?T -> _ => T end in
+  run_template_program
+    (subst <- tmQuote v;;
+     qsubstTy <- tmQuote substTy;;
+     match subst with
+     | tFix [b] _
+       => tmUnquote
+            (tLambda
+               {| binder_name := nNamed "subst'"; binder_relevance := Relevant |}
+               qsubstTy
+               b.(dbody))
+     | _ => tmPrint subst;; tmFail "bad subst body"
+     end)
+    (fun v => lazymatch v with
+              | {| my_projT2 := ?v |} => exact v
+              end).
+Defined.
+
+Definition presubst (subst : list term -> nat -> term -> term) (s : list term) (k : nat) (u : term) : term
+  := if match s with [] => true | _ => false end
+     then u
+     else subst s k u.
+
+Fixpoint subst' s k u {struct u} := subst_step lift_opt (presubst subst') s k u.
+Definition subst_opt s k u := presubst subst' s k u.
+Fixpoint subst'_nolift s k u {struct u} := subst_step (fun _ _ v => v) (presubst subst'_nolift) s k u.
+Definition subst_nolift_opt s k u := presubst subst'_nolift s k u.
+
+Lemma eq_presubst subst s k u
+  : subst s k u = PCUICAst.subst s k u
+    -> presubst subst s k u = PCUICAst.subst s k u.
+Proof.
+  destruct s; cbn; auto.
+  rewrite !subst_empty; reflexivity.
+Qed.
+
+Lemma eq_subst' s k u : subst' s k u = PCUICAst.subst s k u.
+Proof.
+  revert s k; induction u using term_forall_list_ind; intros; cbn -[presubst]; try reflexivity.
+  all: repeat destruct ?; subst.
+  all: rewrite ?eq_lift_opt.
+  all: f_equal.
+  all: repeat first [ progress intros
+                    | reflexivity
+                    | solve [ eauto ]
+                    | rewrite eq_presubst
+                    | apply map_ext_in_iff
+                    | apply map_def_eq_spec
+                    | apply map_predicate_k_eq_spec
+                    | apply map_branch_k_eq_spec
+                    | progress cbv [shiftf] ].
+  all: repeat first [ progress hnf in *
+                    | solve [ eauto ]
+                    | progress rdest
+                    | progress sq
+                    | match goal with
+                      | [ H : All _ _ |- _ ] => pose proof (fun X H' => @All_In _ _ _ X H' H); clear H
+                      | [ H : forall X, In X ?v -> _ |- _ ]
+                        => exactly_once (idtac; multimatch goal with
+                                                | [ H' : In _ v |- _ ]
+                                                  => specialize (H _ H')
+                                                end)
+                      end ].
+Qed.
+
+Lemma eq_subst_opt s k u : subst_opt s k u = PCUICAst.subst s k u.
+Proof.
+  cbv [subst_opt]; rewrite eq_presubst; rewrite ?eq_subst'; reflexivity.
+Qed.
+
+Lemma eq_subst'_nolift s k u
+  (Hs : Forall (fun t => closed t) s)
+  : subst'_nolift s k u = PCUICAst.subst s k u.
+Proof.
+  revert k; induction u using term_forall_list_ind; intros; cbn -[presubst]; try reflexivity.
+  all: repeat destruct ?; subst.
+  all: rewrite ?lift_closed by now eapply Forall_forall in Hs; try eapply nth_error_In; tea.
+  all: f_equal.
+  all: repeat first [ progress intros
+                    | reflexivity
+                    | solve [ eauto ]
+                    | rewrite eq_presubst
+                    | apply map_ext_in_iff
+                    | apply map_def_eq_spec
+                    | apply map_predicate_k_eq_spec
+                    | apply map_branch_k_eq_spec
+                    | progress cbv [shiftf] ].
+  all: repeat first [ progress hnf in *
+                    | solve [ eauto ]
+                    | progress rdest
+                    | progress sq
+                    | match goal with
+                      | [ H : All _ _ |- _ ] => pose proof (fun X H' => @All_In _ _ _ X H' H); clear H
+                      | [ H : forall X, In X ?v -> _ |- _ ]
+                        => exactly_once (idtac; multimatch goal with
+                                                | [ H' : In _ v |- _ ]
+                                                  => specialize (H _ H')
+                                                end)
+                      end ].
+Qed.
+
+Lemma eq_subst_nolift_opt s k u
+  (Hs : Forall (fun t : term => closed t) s)
+  : subst_nolift_opt s k u = PCUICAst.subst s k u.
+Proof.
+  cbv [subst_nolift_opt]; rewrite eq_presubst; rewrite ?eq_subst'_nolift; tea; reflexivity.
+Qed.
+
+(*
+Definition subst_nolift : list term -> nat -> term -> term.
+Proof.
+  let v := (eval cbv delta [subst] in subst) in
+  let v := lazymatch (eval pattern (@lift) in v) with
+           | ?f _ => f
+           end in
+  let v := (eval cbv beta in (v (fun _ _ x => x))) in
+  exact v.
+Defined.
+
+Lemma closed_subst_nolift {cf : config.checker_flags} {Σ}
+  (s : list term)
+  (Γ' : list term)
+  (Hs : All2 (fun t T => Σ ;;; [] |- t : T) s Γ')
+  (wfΣ : wf Σ)
+  : forall u k, subst s k u = subst_nolift s k u.
+Proof.
+  induction u using term_forall_list_ind; intros.
+  all: cbn [subst subst_nolift].
+  all: f_equal.
+  all: repeat
+         unshelve
+         first [ progress intros
+               | progress hnf in *
+               | progress destruct_head'_prod
+               | reflexivity
+               | solve [ eauto ]
+               | progress destruct ?
+               | apply lift_closed
+               | apply map_def_eq_spec
+               | apply map_predicate_k_eq_spec
+               | apply map_branch_k_eq_spec
+               | now change 0 with #|[]:context|; eapply subject_closed
+               | match goal with
+                 | [ H : All _ ?x |- context[map _ ?x] ] => induction H; cbn [map]; congruence
+                 | [ H : All _ ?x |- map (map_def (subst _ _) (subst _ ?k')) ?x = _ ]
+                   => generalize k'; intro; induction H; cbn [map]; f_equal; try congruence
+                 | [ H : nth_error ?s _ = Some _, H' : All2 _ ?s _ |- closedn _ _ = true ]
+                   => eapply All2_nth_error_Some in H; [ | eassumption ]; destruct H as [? [_ ?]]
+                 | [ H : All _ ?x |- context[map _ ?x] ] => induction H; cbn [map]; f_equal; try congruence
+                 end ].
+Qed.
+ *)
+Lemma closed_substitution {cf : config.checker_flags} {Σ : global_env_ext}
+  (s : list term)
+  (Γ' : list term)
+  (t T : term)
+  (wfΣ : wf Σ)
+  (Hs : All2_fold (fun s0 Γ'0 t T => Σ ;;; [] |- t : subst0 s0 T) s Γ')
+  (Γ'' := List.map (fun ty => {| BasicAst.decl_name := {| binder_name := nAnon; binder_relevance := Relevant |} ; BasicAst.decl_body := None ; BasicAst.decl_type := ty |}) Γ')
+  (Ht : Σ ;;; Γ'' |- t : T)
+  : Σ ;;; [] |- subst0 s t : subst0 s T.
+Proof.
+  apply (@substitution cf Σ wfΣ [] Γ'' s [] t T);
+    try (cbn; rewrite app_context_nil_l; assumption).
+  clear Ht t T.
+  subst Γ''; induction Hs; cbn [List.map]; constructor; trivial.
+  (*{ rewrite subst_closedn; [ assumption | ].
+    change 0 with #|[]:context|.
+    eapply @type_closed; eassumption. }*)
+Qed.
+Notation subst0_opt t := (subst_opt t 0).
+Notation subst0_nolift_opt t := (subst_nolift_opt t 0).
+Lemma closed_substitution_opt {cf : config.checker_flags} {Σ : global_env_ext}
+  (s : list term)
+  (Γ' : list term)
+  (t T : term)
+  (wfΣ : wf Σ)
+  (Hs : All2_fold (fun s0 Γ'0 t T => Σ ;;; [] |- t : subst0_nolift_opt s0 T) s Γ')
+  (Γ'' := List.map (fun ty => {| BasicAst.decl_name := {| binder_name := nAnon; binder_relevance := Relevant |} ; BasicAst.decl_body := None ; BasicAst.decl_type := ty |}) Γ')
+  (Ht : Σ ;;; Γ'' |- t : T)
+  : Σ ;;; [] |- subst0_nolift_opt s t : subst0_nolift_opt s T.
+Proof.
+  assert (H : Forall (fun t0 : term => closed t0) s).
+  { clear -Hs wfΣ; induction Hs; constructor; eauto.
+    change 0 with #|[]:context|.
+    eapply @subject_closed; tea. }
+  rewrite !eq_subst_nolift_opt; tea.
+  eapply closed_substitution; tea.
+  clear -Hs H.
+  toAll.
+  induction Hs; constructor; auto.
+  all: match goal with H : All _ (_ :: _) |- _ => inversion H; subst; clear H end.
+  all: rewrite eq_subst_nolift_opt in *; tea; try toAll; eauto.
+Qed.
+
+Fixpoint All2_fold_cps {A} (P : list A -> list A -> A -> A -> Type) (Q : Type) (l1 l2 : list A) {struct l1}
+  := match l1, l2 with
+     | [], [] => Q
+     | [], _ | _, [] => True
+     | x :: xs, y :: ys
+       => P xs ys x y -> All2_fold_cps P Q xs ys
+     end.
+
+#[local] Hint Constructors All2_fold : core.
+Lemma All2_fold_cps_id {A P Q l1 l2}
+  : @All2_fold_cps A P Q l1 l2 <~> (All2_fold P l1 l2 -> Q).
+Proof.
+  split; revert l2; induction l1 as [|?? IH], l2 as [|? l2]; cbn.
+  all: intros.
+  all: try match goal with H : All2_fold _ _ _ |- _ => inversion H; subst end.
+  all: intuition eauto.
+Qed.
+
+Lemma closed_substitution_cps {cf : config.checker_flags} {Σ : global_env_ext}
+  (s : list term)
+  (Γ' : list term)
+  (t T : term)
+  (wfΣ : wf Σ)
+  (Γ'' := List.map (fun ty => {| BasicAst.decl_name := {| binder_name := nAnon; binder_relevance := Relevant |} ; BasicAst.decl_body := None ; BasicAst.decl_type := ty |}) Γ')
+  : All2_fold_cps
+      (fun s0 Γ'0 t T => Σ ;;; [] |- t : subst0_nolift_opt s0 T)
+      ((Σ ;;; Γ'' |- t : T) -> (Σ ;;; [] |- subst0_nolift_opt s t : subst0_nolift_opt s T))
+      s Γ'.
+Proof.
+  apply All2_fold_cps_id; intros; eapply closed_substitution_opt; eassumption.
+Qed.
+
+(*Check All2_fold.*)
+(*
+Lemma closed_substitution_nolift {cf : config.checker_flags} {Σ}
+  (s : list term)
+  (Γ' : list term)
+  (t T : term)
+  (Hs : All2 (fun t T => Σ ;;; [] |- t : T) s Γ')
+  (wfΣ : wf Σ)
+  (Γ'' := List.map (fun ty => {| BasicAst.decl_name := {| binder_name := nAnon; binder_relevance := Relevant |} ; BasicAst.decl_body := None ; BasicAst.decl_type := ty |}) Γ')
+  (Ht : Σ ;;; Γ'' |- t : T)
+  : Σ ;;; [] |- subst_nolift s 0 t : subst_nolift s 0 T.
+Proof.
+  erewrite <- !closed_subst_nolift by eassumption.
+  now eapply @closed_substitution.
+Qed.
+*)
+
+(* generates new version of [t * s], where [s] holds (de Bruijn index, quoted term, unquoted term, unquoted type) *)
+Definition precollect_constants_k
+  (collect_constants_k : nat -> term -> StateT (list (nat * term * term * term)) TemplateMonad term)
+  (collect_constants_k_from_fix : nat -> term -> StateT (list (nat * term * term * term)) TemplateMonad term)
+  (offset : nat) (t : term)
+  : StateT (list (nat * term * term * term)) TemplateMonad term
+  := qt <- State.lift (tmQuote t);;
+     let '(qh, qargs) := decompose_app qt in
+     rv <- match qh, qargs with
+           | tRel _, _
+           | tVar _, _
+           | tEvar _ _, _
+           | tConst _ _, _
+             => s <- State.get;;
+                match find (fun '(i, qv, v, vT) => qt == qv) s with
+                | Some (i, qv, v, vT)
+                  => i' <- State.lift (tmEval cbv (offset + i));;
+                     ret (Some (tRel i'))
+                | None
+                  => vT <- State.lift (let tc := tmInferInstance None (infer_type_of t) in
+                                       inst <- tc;;
+                                       match inst with
+                                       | my_Some vT => ret vT
+                                       | my_None
+                                         => tmPrint (t, qt, qh, qargs);;
+                                            tmPrint tc;;
+                                            tmFail "precollect_constants_k: could not infer instance"
+                                       end);;
+                     _ <- collect_constants_k_from_fix 0 vT;;
+                     s <- State.get;;
+                     i <- State.lift (tmEval cbv (List.length s));;
+                     i' <- State.lift (tmEval cbv (offset + i));;
+                     State.set ((i, qt, t, vT) :: s);;
+                     ret (Some (tRel i'))
+                end
+           | tApp _ _, _
+             => State.lift (tmPrint qt;; tmFail "decompose_app should not return tApp")
+           | tConstruct _ _ _, _
+             => ret None
+           | _, _
+             => State.lift (tmPrint qt;; tmPrint (qh, qargs);; tmFail "collect_constants: requires constructor tree or tRel, tVar, tEvar, tConst")
+           end;;
+     match rv with
+     | Some rv => ret rv
+     | None
+       => collect_constants_k offset t
+     end.
+
+
+Fixpoint collect_constants_k'
+  (collect_constants_k_from_fix : nat -> term -> StateT _ TemplateMonad term)
+  (offset : nat) (t : term)
+  : StateT _ TemplateMonad term
+  := let collect_constants_k := precollect_constants_k (collect_constants_k' collect_constants_k_from_fix) collect_constants_k_from_fix in
+     match t with
+     | tRel _
+     | tVar _
+     | tSort _
+     | tProj _ _
+     | tPrim _
+     | tConst _ _
+     | tInd _ _
+     | tConstruct _ _ _
+       => ret t
+     | tEvar n l
+       => l <- monad_map (collect_constants_k offset) l;;
+          ret (tEvar n l)
+     | tProd na A B
+       => A <- collect_constants_k offset A;;
+          B <- collect_constants_k (S offset) B;;
+          ret (tProd na A B)
+     | tLambda na A t
+       => A <- collect_constants_k offset A;;
+          t <- collect_constants_k (S offset) t;;
+          ret (tLambda na A t)
+     | tLetIn na b B t
+       => b <- collect_constants_k offset b;;
+          B <- collect_constants_k offset B;;
+          t <- collect_constants_k (S offset) t;;
+          ret (tLetIn na b B t)
+     | tApp u v
+       => u <- collect_constants_k offset u;;
+          v <- collect_constants_k offset v;;
+          ret (tApp u v)
+     | tCase indn p c brs
+       => p <- monad_map_predicate_k ret collect_constants_k offset p;;
+          c <- collect_constants_k offset c;;
+          brs <- monad_map_branches_k collect_constants_k ret offset brs;;
+          ret (tCase indn p c brs)
+     | tFix mfix idx
+       => mfix <- monad_map (monad_map_def (collect_constants_k offset) (collect_constants_k offset)) mfix;;
+          ret (tFix mfix idx)
+     | tCoFix mfix idx
+       => mfix <- monad_map (monad_map_def (collect_constants_k offset) (collect_constants_k offset)) mfix;;
+          ret (tCoFix mfix idx)
+     end.
+
+Definition collect_constants_k : nat -> term -> StateT (list (nat * term * term * term)) TemplateMonad term
+  := fun n t st
+     => tmFix (fun collect_constants_k_from_fix '(n, t, st)
+               => let collect_constants_k_from_fix n t st := collect_constants_k_from_fix (n, t, st) in
+                  precollect_constants_k (collect_constants_k' collect_constants_k_from_fix) collect_constants_k_from_fix n t st)
+              (n, t, st).
+Notation collect_constants := (collect_constants_k 0).
+
+Definition List_map_alt {A} {B} := Eval cbv in @List.map A B.
+Definition List_rev_alt {A} := Eval cbv in @rev A.
+
+Fixpoint redo_types_and_indices' (ls : list (nat * term * term * term))
+  : StateT _ TemplateMonad (list (nat * term * term * term))
+  := match ls with
+     | [] => ret []
+     | (_, qv, v, vT) :: ls
+       => State.set ls;;
+          ls <- redo_types_and_indices' ls;;
+          State.set ls;;
+          vT <- collect_constants_k 0 vT;;
+          ls <- monad_map (fun '(i, qt, t, vT) => ret (S i, qt, t, vT)) ls;;
+          State.set ls;;
+          ret ((0, qv, v, vT) :: ls)
+     end.
+
+Definition evalStateT {S M T} {TM : Monad M} (p : StateT S M T) (st : S) : M T
+  := '(v, st) <- p st;;
+     ret v.
+
+Definition redo_types_and_indices (ls : list (nat * term * term * term)) : TemplateMonad (list (nat * term * term * term))
+  := evalStateT (redo_types_and_indices' ls) ls.
+
+Definition collect_constants_build_substituition (t : term) (T : term)
+  : TemplateMonad (term (* t *) * term (* T *) * list term (* s *) * list term (* Γ *) )
+  := qmap <- tmQuoteToGlobalReference (@List_map_alt);;
+     qmap <- match kername_of_global_reference qmap with
+             | Some kn => ret kn
+             | None => tmPrint qmap;; tmFail "no List_map_alt"
+             end;;
+     qrev <- tmQuoteToGlobalReference (@List_rev_alt);;
+     qrev <- match kername_of_global_reference qrev with
+             | Some kn => ret kn
+             | None => tmPrint qrev;; tmFail "no List_rev_alt"
+             end;;
+     '(T', st) <- collect_constants T [];;
+     '(t', st) <- collect_constants t st;;
+     st <- redo_types_and_indices st;;
+     T' <- evalStateT (collect_constants T) st;;
+     t' <- evalStateT (collect_constants t) st;;
+     T' <- tmEval cbv T';;
+     t' <- tmEval cbv t';;
+     st <- tmEval hnf st;;
+     (*tmPrint st;;*)
+     s <- tmEval (unfold qmap) (List_map_alt (fun '(i, qv, v, vT) => v) st);;
+     Γ <- tmEval (unfold qmap) (List_map_alt (fun '(i, qv, v, vT) => vT) st);;
+     ret (t', T', s, Γ).
+  (*
+  (cf : config.checker_flags) (Σ : global_env_ext)
+closed_substitution {cf : config.checker_flags} {Σ}
+  (s : list term)
+  (Γ' : list term)
+  (t T : term)
+  (Hs : All2_fold (fun s0 Γ'0 t T => Σ ;;; [] |- t : subst0 s0 T) s Γ')
+  (wfΣ : wf Σ)
+  (Γ'' := List.map (fun ty => {| BasicAst.decl_name := {| binder_name := nAnon; binder_relevance := Relevant |} ; BasicAst.decl_body := None ; BasicAst.decl_type := ty |}) Γ')
+  (Ht : Σ ;;; Γ'' |- t : T)
+  : Σ ;;; [] |- subst0 s t : subst0 s T.
+Proof.
+*)
+(*
+
+Definition replace_typing_for_safechecker (cf : config.checker_flags) Σ t T
+  : TemplateMonad (@typing cf Σ [] t T).
+  Print infer_quotation_of_well_typed.
+  refine (let collect_all_constants := (T' <- collect_constants T;;
+                                        t' <- collect_constants t;;
+                                        ret (t', T')) in
+          '((t', T'), Γ') <- collect_all_constants [];;
+          let Γ' := map (fun '(_, _, t) => t) Γ' in
+          tys <- monad_map
+                   (fun t
+                    => let tc := infer_quotation_of_well_typed t in
+                       inst <- tmInferInstance None tc;;
+                       match inst with
+                       | my_Some v => ret v
+                       | my_None => tmPrint tc;; tmFail "could not find instance"
+                       end)
+                   Γ';;
+          _).
+
+  infer_quotation_of_well_typed
+ *)
+(*From MetaCoq.PCUIC Require Import PCUICEquality PCUICAst PCUICReflect PCUICSafeLemmata PCUICTyping PCUICNormal PCUICAstUtils PCUICSN.
+
+From MetaCoq.SafeChecker Require Import PCUICEqualityDec PCUICWfReduction PCUICErrors PCUICSafeReduce PCUICTypeChecker PCUICSafeChecker PCUICWfEnv PCUICWfEnvImpl PCUICSafeConversion.
+Locate Module PCUICWfEnvImpl.
+
+*)
+#[local,program] Instance quotation_fake_abstract_guard_impl : PCUICWfEnvImpl.abstract_guard_impl :=
+  {
+    guard_impl := PCUICWfEnvImpl.fake_guard_impl
+  }.
+Next Obligation. todo "this axiom is inconsitent, only used to make infer compute". Qed.
+#[local,program] Instance assume_normalization {cf nor} : @PCUICSN.Normalization cf nor.
+Next Obligation. todo "we should write a Template Monad program to prove normalization for the particular program being inferred, rather than axiomatizing it". Qed.
+#[local] Existing Instance PCUICSN.normalization.
+
+Check @check.
+Print typing_result_comp.
 
 Variant quotation_check_error :=
   | QTypeError (_ : type_error)
   | QConfigNotNormalizing (cf : config.checker_flags)
-  | QEnvError   (_ : env_error)
+  | QEnvError (*(_ : wf_env_ext)*) (_ : env_error)
   | QContextTypeError (_ : type_error)
 .
 
-Definition quotation_check (cf : config.checker_flags) (Σ : global_env_ext) (Γ : context) (t T : term) : option quotation_check_error.
-Admitted.
-Lemma quotation_check_valid {cf Σ Γ t T} : quotation_check cf Σ Γ t T = None -> @wf_ext cf Σ * wf_local Σ Γ * @typing cf Σ Γ t T.
-Admitted.
-Definition universes_of_Instance (t : Instance.t) (acc : LevelSet.t) : LevelSet.t.
-Admitted.
-Definition universes_of_universe (t : Universe.t) (acc : LevelSet.t) : LevelSet.t.
-Admitted.
-Definition universes_of_prim_val {A} (universes_of_term' : A -> StateT LevelSet.t TemplateMonad A) (t : PCUICPrimitive.prim_val A) : StateT LevelSet.t TemplateMonad (PCUICPrimitive.prim_val A).
-admit.
+(* TODO: move? *)
+Definition dec_normalizing cf : {@PCUICSN.normalizing_flags cf} + {~@PCUICSN.normalizing_flags cf}.
+Proof.
+  destruct cf.(config.check_univs) eqn:?; [ | right ].
+  all: try left.
+  all:
+    abstract
+      (first [ constructor | destruct 1 ]; destruct cf; cbv in *; subst; congruence).
 Defined.
+
+Definition quotation_check (cf : config.checker_flags) (Σ : global_env_ext) (Γ : context) (t T : term) : option quotation_check_error.
+Proof.
+  destruct (dec_normalizing cf); [ | exact (Some (QConfigNotNormalizing cf)) ].
+  simple refine (let cwf := @check_wf_ext cf _ optimized_abstract_env_impl Σ _ in
+                 match cwf with
+                 | CorrectDecl (exist A pf)
+                   => let wfΣ := abstract_env_ext_wf (abstract_env_prop:=optimized_abstract_env_prop) _ pf in
+                      let X := @build_wf_env_ext cf _ Σ wfΣ in
+                      let cwfΓ := @check_wf_local cf _ optimized_abstract_env_impl X _ Γ in
+                      match cwfΓ with
+                      | Checked wfΓ
+                        => let c := typing_error_forget (@check cf _ optimized_abstract_env_impl X _ Γ wfΓ t T) in
+                           match c with
+                           | Checked _ => None
+                           | TypeError t => Some (QTypeError t)
+                           end
+                      | TypeError t => Some (QContextTypeError t)
+                      end
+                 | EnvError st err
+                   => Some (QEnvError (*st*) err)
+                 end).
+Defined.
+Lemma quotation_check_valid {cf Σ Γ t T} : quotation_check cf Σ Γ t T = None -> @wf_ext cf Σ * wf_local Σ Γ * @typing cf Σ Γ t T.
+Proof.
+  cbv [quotation_check].
+  repeat destruct ?; subst;
+    lazymatch goal with
+    | [ |- None = None -> _ ] => intros _
+    | [ |- Some _ = None -> _ ] => congruence
+    end.
+  match goal with
+  | [ |- ?P ] => cut (∥ @wf_ext cf Σ * wf_local Σ Γ * @typing cf Σ Γ t T ∥)
+  end.
+  { todo "Find a way to get the safechecker to produce unsquashed judgments". }
+  lazymatch goal with
+  | [ H : _ = CorrectDecl _ (exist _ ?pf) |- _ ]
+    => pose proof (abstract_env_ext_wf (abstract_env_prop:=optimized_abstract_env_prop) _ pf)
+  end.
+  repeat match goal with
+         | [ H : _ |- _ ] => unique pose proof (H _ eq_refl)
+         end.
+  sq; auto.
+Qed.
+
+Ltac handle_typing_by_factoring _ :=
+  let H := fresh in
+  lazymatch goal with
+  | [ |- @typing ?cf ?Σ ?Γ ?t ?T ]
+    => run_template_program
+         (collect_constants_build_substituition t T)
+         (fun v
+          => lazymatch v with
+             | (?t', ?T', ?s', ?Γ')
+               => pose proof (@closed_substitution_cps cf Σ s' Γ' t' T') as H;
+                  cbv [All2_fold_cps] in H
+             | ?v => fail 0 "invalid collect_constants_build_substituition ret" v
+             end)
+  end;
+  simple apply H; clear H; tea;
+  cbv [subst_nolift_opt presubst subst'_nolift subst_step] in *;
+  cbn [Nat.sub List.length nth_error Nat.leb] in *.
+
+Ltac handle_typing_by_tc _ :=
+  lazymatch goal with
+  | [ |- @typing ?cf (?Σ, Monomorphic_ctx) [] ?t ?T ]
+    => notypeclasses refine (@typing_quoted_term_of_general_empty_ctx _ _ _ _ T t _ cf Σ _ _ _ _);
+       [ typeclasses eauto | .. ]
+  | [ |- ?G ]
+    => fail 0 "Not typing goal" G
+  end.
+
+Ltac handle_typing_tc_side_conditions_step _ :=
+  match goal with
+  | [ |- extends ?x ?x ] => apply extends_refl
+  | [ |- extends ?x (merge_global_envs ?y ?z) ]
+    => lazymatch z with
+       | context[x] => transitivity z; [ | apply extends_r_merge ]
+       | _
+         => lazymatch y with
+            | x => try exact _
+            | context[x] => transitivity y; [ | apply extends_l_merge ]
+            | _ => idtac
+            end
+       end
+  | [ |- is_true (config.impl ?x ?x) ]
+    => apply config.impl_refl
+  | [ |- is_true (config.impl ?x (config.union_checker_flags ?y ?z)) ]
+    => lazymatch z with
+       | context[x]
+         => apply (@config.impl_trans x z (config.union_checker_flags y z));
+            [ | apply config.union_checker_flags_spec ]
+       | _
+         => lazymatch y with
+            | context[x]
+              => apply (@config.impl_trans x y (config.union_checker_flags y z));
+                 [ | apply config.union_checker_flags_spec ]
+            | _ => idtac
+            end
+       end
+  | [ |- wf _ ] => try assumption
+  | [ H : context[compatibleb ?x ?y] |- compatible ?x ?y ]
+    => destruct (@compatibleP x y); [ assumption | clear -H; try congruence ]
+  end.
+Ltac handle_typing_tc_side_conditions _ := repeat handle_typing_tc_side_conditions_step ().
+
+Ltac handle_typing_by_safechecker0 cf0 Σ0 :=
+  lazymatch goal with
+  | [ |- @typing ?cf ?Σ ?Γ ?t ?T ]
+    => destruct (@quotation_check_valid cf0 Σ0 Γ t T)
+  | [ |- ?G ] => fail 0 "Not a typing goal:" G
+  end;
+  [ | destruct_head'_prod ].
+Ltac handle_typing_by_safechecker_sc1 := vm_compute; try reflexivity.
+Ltac handle_typing_by_safechecker_sc2 cf0 Σ0 :=
+  let cf := match goal with |- @typing ?cf _ _ _ _ => cf end in
+  eapply (@weakening_env cf Σ0); tea;
+  try eapply (@weakening_config_wf cf0);
+  try eapply (@weakening_config cf0);
+  try apply config.strictest_checker_flags_strictest; (* heuristic *)
+  try apply wf_ext_wf;
+  try assumption;
+  try exact _.
+
+Ltac handle_typing_by_safechecker' cf0 Σ0 :=
+  handle_typing_by_safechecker0 cf0 Σ0;
+  [ | handle_typing_by_safechecker_sc2 cf0 Σ0 ].
+
+Ltac handle_typing_by_safechecker cf0 Σ0 :=
+  handle_typing_by_safechecker0 cf0 Σ0;
+  [ handle_typing_by_safechecker_sc1
+  | handle_typing_by_safechecker_sc2 cf0 Σ0 ].
+
+Definition universes_of_Instance (t : Instance.t) (acc : LevelSet.t) : LevelSet.t
+  := fold_right LevelSet.add acc t.
+Definition universes_of_LevelExprSet (t : LevelExprSet.t) (acc : LevelSet.t) : LevelSet.t
+  := fold_right LevelSet.add acc (List.map fst (LevelExprSet.elements t)).
+Definition universes_of_LevelAlgExpr (t : LevelAlgExpr.t) (acc : LevelSet.t) : LevelSet.t
+  := universes_of_LevelExprSet (t.(t_set)) acc.
+Definition universes_of_universe (t : Universe.t) (acc : LevelSet.t) : LevelSet.t
+  := match t with
+     | Universe.lProp => acc
+     | Universe.lSProp => acc
+     | Universe.lType l => universes_of_LevelAlgExpr l acc
+     end.
+
+Definition universes_of_prim_model {A} (universes_of_term' : A -> StateT LevelSet.t TemplateMonad A) {tg} (t : PCUICPrimitive.prim_model A tg) : StateT LevelSet.t TemplateMonad (PCUICPrimitive.prim_model A tg)
+  := match t with
+     | primIntModel _
+     | primFloatModel _
+       => ret t
+     end.
+Definition universes_of_prim_val {A} (universes_of_term' : A -> StateT LevelSet.t TemplateMonad A) (t : PCUICPrimitive.prim_val A) : StateT LevelSet.t TemplateMonad (PCUICPrimitive.prim_val A)
+  := _ <- universes_of_prim_model universes_of_term' t.π2;;
+     ret t.
 
 Definition preuniverses_of_partial_term
   (universes_of_term : term -> StateT LevelSet.t TemplateMonad term)
@@ -232,13 +914,17 @@ Definition preuniverses_of_partial_term
      | None
        => universes_of_term t
      end.
-Definition monad_map_universes {A} (f : A -> LevelSet.t -> LevelSet.t) (t : A) : StateT LevelSet.t TemplateMonad A.
-exact (acc <- State.get;;
+
+Definition visit_universes (univs : LevelSet.t) : StateT LevelSet.t TemplateMonad unit
+  := State.update (fun acc => LevelSet.union acc univs).
+
+Definition monad_map_universes {A} (f : A -> LevelSet.t -> LevelSet.t) (t : A) : StateT LevelSet.t TemplateMonad A
+  := acc <- State.get;;
      State.set (f t acc);;
-     ret t).
-Defined.
-Fixpoint universes_of_term' (t : term) : StateT LevelSet.t TemplateMonad term.
-exact (let universes_of_term := preuniverses_of_partial_term universes_of_term' in
+     ret t.
+
+Fixpoint universes_of_term' (t : term) : StateT LevelSet.t TemplateMonad term
+  := let universes_of_term := preuniverses_of_partial_term universes_of_term' in
      match t with
      | tRel _
      | tVar _
@@ -284,22 +970,39 @@ exact (let universes_of_term := preuniverses_of_partial_term universes_of_term' 
           _ <- universes_of_term c;;
           _ <- monad_map_branches universes_of_term (monad_map_context universes_of_term) brs;;
           ret t
-     end).
-Defined.
-Definition universes_of_partial_term (t : term) : StateT LevelSet.t TemplateMonad LevelSet.t.
-exact (preuniverses_of_partial_term universes_of_term' t;; State.get).
-Defined.
-Definition universes_of_type_of_quotation_of_well_typed' {cf Σ T t qT qt} (_ : @quotation_of_well_typed cf Σ T t qT qt) : TemplateMonad LevelSet.t.
-exact (v <- evalStateT (universes_of_partial_term qT;; universes_of_partial_term qt) LevelSet.empty;;
-     tmEval cbv v).
-Defined.
+     end.
+
+Definition universes_of_partial_term (t : term) : StateT LevelSet.t TemplateMonad LevelSet.t
+  := preuniverses_of_partial_term universes_of_term' t;; State.get.
+
+Definition get_universes_of_partial_term (t : term) : TemplateMonad LevelSet.t
+  := evalStateT (universes_of_partial_term t) LevelSet.empty.
+
+Definition universes_of_type_of_quotation_of_well_typed' {cf Σ T t qT qt} (_ : @quotation_of_well_typed cf Σ T t qT qt) : TemplateMonad LevelSet.t
+  := v <- evalStateT (universes_of_partial_term qT;; universes_of_partial_term qt) LevelSet.empty;;
+     tmEval cbv v.
 Notation universes_of_type_of_quotation_of_well_typed qty
   := (match qty return _ with
       | qtyv
         => ltac:(run_template_program (universes_of_type_of_quotation_of_well_typed' qtyv) (fun v => exact v))
       end) (only parsing).
-Definition merge_universe_levels (Σ : global_env_ext) (univs : LevelSet.t) : global_env_ext.
-Admitted.
+
+Definition merge_universes_env (Σ : global_env) (univs : ContextSet.t) : global_env
+  := {| universes := ContextSet.union Σ.(universes) univs
+     ; declarations := Σ.(declarations)
+     ; retroknowledge := Σ.(retroknowledge) |}.
+
+Definition merge_universe_levels_env (Σ : global_env) (univs : LevelSet.t) : global_env
+  := {| universes := (LevelSet.union Σ.(universes).1 univs, Σ.(universes).2)
+     ; declarations := Σ.(declarations)
+     ; retroknowledge := Σ.(retroknowledge) |}.
+
+Definition merge_universes (Σ : global_env_ext) (univs : ContextSet.t) : global_env_ext
+  := (merge_universes_env Σ univs, Σ.2).
+Definition merge_universe_levels (Σ : global_env_ext) (univs : LevelSet.t) : global_env_ext
+  := (merge_universe_levels_env Σ univs, Σ.2).
+Axiom proof_admitted : False.
+Ltac admit := abstract case proof_admitted.
 #[export] Instance well_typed_ground_quotable_of_bp
   {b P} (H : b = true -> P)
   {qH : quotation_of H} (H_for_safety : P -> b = true)
@@ -320,5 +1023,705 @@ Admitted.
 Proof.
   subst Σ0'.
   intros t wfΣ.
-  Time  (intros; lazymatch goal with |- @typing ?cf ?Σ ?Γ ?t ?T => pose proof (@quotation_check_valid config.strictest_checker_flags Σ0 Γ t T) as H' end; clear H'; admit).
-Time Timeout 1 Qed.
+  Time  (intros; lazymatch goal with |- @typing ?cf ?Σ ?Γ ?t ?T => pose proof (@quotation_check_valid config.strictest_checker_flags Σ0 Γ t T) as H' end; clear H'; admit). Time Timeout 1 Qed.
+  handle_typing_by_factoring ().
+  all: [ > handle_typing_by_tc () .. | ].
+  all: subst Σ.
+  all: [ > handle_typing_tc_side_conditions () .. | ].
+  all: [ > ].
+  repeat match goal with H : _ |- _ => revert H end.
+  match goal with |- ?T => refine (@id T _) end.
+
+
+Finished transaction in 0.161 secs (0.161u,0.s) (successful)
+                              Finished transaction in 0.2 secs (0.2u,0.s) (successful)
+Finished transaction in 0.195 secs (0.195u,0.s) (successful)
+                              Finished transaction in 7.062 secs (7.062u,0.s) (successful)
+Finished transaction in 0.116 secs (0.116u,0.s) (successful)
+
+         pose
+  Time admit. Time Qed.
+Finished transaction in 0.053 secs (0.053u,0.s) (successful)
+                              Finished transaction in 0.17 secs (0.17u,0.s) (successful)
+  Time abstract (intros; handle_typing_by_safechecker config.strictest_checker_flags Σ0).
+  Time Qed.
+  all: todo "foo". Qed.
+
+  todo "foo".
+Qed.
+
+  Search compatible compatibleb.
+  2: apply extends_refl.
+  2: etransitivity
+  Search extends merge_global_envs.
+  2: apply extends_m
+  all: try assumption.
+  all: subst
+  all: lazymatch goal iwth
+  Set Printing Implicit.
+  exact _.
+  end.
+  end.
+  run_template_program p (fun v => pose v as v').
+  Lemma closed_substitution_cps {cf : config.checker_flags} {Σ : global_env_ext}
+  (s : list term)
+  (Γ' : list term)
+  (t T : term)
+  (wfΣ : wf Σ)
+
+
+  closed_substitution_nolift {cf : config.checker_flags} {Σ}
+  (s : list term)
+  (Γ' : list term)
+  (t T : term)
+  (Hs : All2 (fun t T => Σ ;;; [] |- t : T) s Γ')
+  (wfΣ : wf Σ)
+  (Γ'' := List.map (fun ty => {| BasicAst.decl_name := {| binder_name := nAnon; binder_relevance := Relevant |} ; BasicAst.decl_body := None ; BasicAst.decl_type := ty |}) Γ')
+  (Ht : Σ ;;; Γ'' |- t : T)
+  : Σ ;;; [] |- subst_nolift s 0 t : subst_nolift s 0 T.
+Proof.
+  erewrite <- !closed_subst_nolift by eassumption.
+  now eapply @closed_substitution.
+Qed.
+  cbn in p0.
+    => run_template_program (collect_constants t []) (fun v => pose v)
+  end.
+
+  Search typing subst.
+  Set Printing Implicit.
+  Print context_decl.
+  Print BasicAst.context_decl.
+  Print aname.
+  Print binder_annot.
+  Check @substitution.
+  epose (@substitution cf Σ Hwf []
+           [{| BasicAst.decl_name := {| binder_name := nAnon; binder_relevance := Relevant |} ; BasicAst.decl_body := None ; BasicAst.decl_type := ltac:(lazymatch type of qtyH with @quotation_of_well_typed _ _ _ ?T _ => exact T end) |};
+            {| BasicAst.decl_name := {| binder_name := nAnon; binder_relevance := Relevant |} ; BasicAst.decl_body := None ; BasicAst.decl_type := ltac:(lazymatch type of qtyP with @quotation_of_well_typed _ _ _ ?T _ => exact T end) |}] [qH; qP] []
+        (tApp (tRel 0)
+       (tApp
+          (tApp
+             (tConstruct
+                {|
+                  inductive_mind := (MPfile ["Logic"; "Init"; "Coq"], "eq");
+                  inductive_ind := 0
+                |} 0 [])
+             (tInd
+                {|
+                  inductive_mind := (MPfile ["Datatypes"; "Init"; "Coq"], "bool");
+                  inductive_ind := 0
+                |} []))
+          (tConstruct
+             {|
+               inductive_mind := (MPfile ["Datatypes"; "Init"; "Coq"], "bool");
+               inductive_ind := 0
+             |} 0 [])))
+        (tRel 1)
+        ) as v.
+  clearbody v.
+  cbn in v.
+  rewrite !lift_closed in v.
+  cbv [subst_context] in v.
+  cbv [fold_context_k] in v.
+  cbn in v.
+  apply v.
+  { constructor.
+    constructor.
+    constructor.
+    all: rewrite !subst_closedn.
+    3: apply qtyH.
+    1:apply qtyP.
+    all: try assumption.
+    all: try solve [ constructor ].
+    change (closedn 0) with (closedn #|[]:context|).
+    eapply type_closed.
+    eapply qtyH.
+    all: try eassumption.
+    now constructor. }
+    apply closedn_
+            eapply
+    3: { move qtyH at bottom.
+         hnf in qtyH.
+         Unset Printing Implicit.
+    2: apply qtyH.
+    all: cbv [subst0]; cbn.
+    2: {
+  Unset Printing Implicit.
+  Print aname.
+  Check {| binder_name := nAnon; binder_relevance := Relevant |} : aname.
+  Check nAnon.
+  Search closedn lift.
+  Print lift0.
+  all: repeat
+         repeat first [ assumption
+                    | now constructor
+                    | progress cbv [subst1] in *
+                    | rewrite subst_closedn
+                    | progress cbn [List.app ind_type]
+                    | progress cbn [subst_instance subst_instance_constr subst_instance_univ]
+                    | progress cbn [type_of_constructor]
+                    | progress cbv [PCUICLookup.declared_minductive_gen]
+                    | match goal with
+                      | [ |- _;;;_ |- tApp _ _ : _ ] => eapply type_App
+                      | [ |- _;;;_ |- tInd _ _ : _ ] => eapply type_Ind
+                      | [ |- _;;;_ |- tConstruct _ _ _ : _ ] => eapply type_Construct
+                      | [ H : @quotation_of_well_typed _ _ _ _ ?qP  |- _;;;_ |- ?qP : _ ]
+                        => (idtac + eapply type_Cumul); [ eapply H | .. ]
+                      | [ H : @quotation_of_well_typed _ _ _ _ ?qP  |- is_true (closedn 0 ?qP) ]
+                        => eapply @subject_closed with (Γ:=[]); [ | eapply H ]; tea
+                      | [ |- wf_local _ [] ] => constructor
+                      | [ |- wf_local _ (_ ,, _) ] => constructor
+                      | [ |- _;;;_ |- tProd _ _ _ : _ ] => eapply type_Prod
+                      | [ |- _;;;_ |- tSort _ : _ ] => eapply type_Sort
+                      | [ |- lift_typing _ _ _ _ _ ] => hnf; try eexists
+                      | [ |- context[tApp ?f ?x] ]
+                        => change (tApp f x) with (mkApps f [x])
+                      | [ |- context[mkApps (mkApps ?f ?x) ?y] ]
+                        => change (mkApps (mkApps f x) y) with (mkApps f (x ++ y))
+                      | [ |- _;;;_ |- mkApps _ _ : _ ]
+                        => eapply type_mkApps
+                      | [ |- PCUICArities.typing_spine _ _ _ _ _ ]
+                        => econstructor
+                      | [ |- declared_inductive _ _ _ _ ] => eapply declared_inductive_from_gen; constructor; hnf
+                      | [ |- declared_constructor _ _ _ _ _ ] => eapply declared_constructor_from_gen; repeat apply conj
+                      | [ |- isType _ _ (tProd _ _ _) ] => apply isType_tProd; split
+                      | [ |- isType _ _ (tSort _) ] => apply isType_Sort
+                      | [ |- _ = _ ] => eassumption
+                      | [ |- _;;;_ |- tSort _ <=s tSort _ ] => apply cumul_Sort
+                      end ].
+  all: lazymatch goal with
+       | [ |- isType _ _ _ ] => cbn; econstructor
+       | [ |- wf_universe _ _ ] => idtac
+       | _ => cbn
+       end.
+  all: repeat
+         repeat first [ assumption
+                      | reflexivity
+                    | progress cbv [subst1] in *
+                    | rewrite subst_closedn
+                    | progress cbn [List.app ind_type]
+                    | progress cbn [subst_instance subst_instance_constr subst_instance_univ]
+                    | progress cbn [type_of_constructor]
+                    | progress cbv [PCUICLookup.declared_minductive_gen]
+                    | match goal with
+                      | [ |- context[tApp ?f ?x] ]
+                        => change (tApp f x) with (mkApps f [x])
+                      | [ |- context[mkApps (mkApps ?f ?x) ?y] ]
+                        => change (mkApps (mkApps f x) y) with (mkApps f (x ++ y))
+                      | [ |- _;;;_ |- mkApps _ _ : _ ]
+                        => eapply type_mkApps
+                      | [ |- _;;;_ |- tInd _ _ : _ ] => eapply type_Ind
+                      | [ |- _;;;_ |- tConstruct _ _ _ : _ ] => eapply type_Construct
+                      | [ |- _;;;_ |- tRel _ : _ ] => (idtac + eapply type_Cumul); [ eapply type_Rel | .. ]
+                      | [ H : @quotation_of_well_typed _ _ _ _ ?qP  |- _;;;_ |- ?qP : _ ]
+                        => (idtac + eapply type_Cumul); [ eapply H | .. ]
+                      | [ H : @quotation_of_well_typed _ _ _ _ ?qP  |- is_true (closedn 0 ?qP) ]
+                        => eapply @subject_closed with (Γ:=[]); [ | eapply H ]; tea
+                      | [ |- wf_local _ [] ] => constructor
+                      | [ |- wf_local _ (_ ,, _) ] => constructor
+                      | [ |- _;;;_ |- tProd _ _ _ : _ ] => eapply type_Prod
+                      | [ |- _;;;_ |- tSort _ : _ ] => eapply type_Sort
+                      | [ |- lift_typing _ _ _ _ _ ] => hnf; try eexists
+                      | [ |- PCUICArities.typing_spine _ _ _ _ _ ]
+                        => econstructor
+                      | [ |- declared_inductive _ _ _ _ ] => eapply declared_inductive_from_gen; constructor; hnf
+                      | [ |- declared_constructor _ _ _ _ _ ] => eapply declared_constructor_from_gen; repeat apply conj
+                      | [ |- isType _ _ (tProd _ _ _) ] => apply isType_tProd; split
+                      | [ |- isType _ _ (tSort _) ] => apply isType_Sort
+                      | [ |- _ = _ ] => eassumption
+                      | [ |- _;;;_ |- tSort _ <=s tSort _ ] => apply cumul_Sort
+                      end ].
+
+  all: lazymatch goal with
+       | [ |- isType _ _ _ ] => cbn; econstructor
+       | [ |- wf_universe _ _ ] => idtac
+       | _ => cbn
+       end.
+  all: repeat
+         repeat first [ assumption
+                      | reflexivity
+                    | progress cbv [subst1] in *
+                    | rewrite subst_closedn
+                    | progress cbn [List.app ind_type]
+                    | progress cbn [subst_instance subst_instance_constr subst_instance_univ]
+                      | progress cbn [type_of_constructor]
+                      | progress cbn [lift0 decl_type vass]
+                    | progress cbv [PCUICLookup.declared_minductive_gen]
+                    | match goal with
+                      | [ |- context[tApp ?f ?x] ]
+                        => change (tApp f x) with (mkApps f [x])
+                      | [ |- context[mkApps (mkApps ?f ?x) ?y] ]
+                        => change (mkApps (mkApps f x) y) with (mkApps f (x ++ y))
+                      | [ |- _;;;_ |- mkApps _ _ : _ ]
+                        => eapply type_mkApps
+                      | [ |- _;;;_ |- tInd _ _ : _ ] => (idtac + eapply type_Cumul); [ eapply type_Ind | .. ]
+                      | [ |- _;;;_ |- tConstruct _ _ _ : _ ] => eapply type_Construct
+                      | [ |- _;;;_ |- tRel _ : _ ] => (idtac + eapply type_Cumul); [ eapply type_Rel | .. ]
+                      | [ H : @quotation_of_well_typed _ _ _ _ ?qP  |- _;;;_ |- ?qP : _ ]
+                        => (idtac + eapply type_Cumul); [ eapply H | .. ]
+                      | [ H : @quotation_of_well_typed _ _ _ _ ?qP  |- is_true (closedn 0 ?qP) ]
+                        => eapply @subject_closed with (Γ:=[]); [ | eapply H ]; tea
+                      | [ |- wf_local _ [] ] => constructor
+                      | [ |- wf_local _ (_ ,, _) ] => constructor
+                      | [ |- _;;;_ |- tProd _ _ _ : _ ] => eapply type_Prod
+                      | [ |- _;;;_ |- tSort _ : _ ] => eapply type_Sort
+                      | [ |- lift_typing _ _ _ _ _ ] => hnf; try eexists
+                      | [ |- PCUICArities.typing_spine _ _ _ _ _ ]
+                        => econstructor
+                      | [ |- declared_inductive _ _ _ _ ] => eapply declared_inductive_from_gen; constructor; hnf
+                      | [ |- declared_constructor _ _ _ _ _ ] => eapply declared_constructor_from_gen; repeat apply conj
+                      | [ |- isType _ _ (tProd _ _ _) ] => apply isType_tProd; split
+                      | [ |- isType _ _ (tSort _) ] => apply isType_Sort
+                      | [ |- _ = _ ] => eassumption
+                      | [ |- _;;;_ |- tSort _ <=s tSort _ ] => apply cumul_Sort
+                      end ].
+  all: lazymatch goal with
+       | [ |- wf_universe _ _ ] => shelve
+       | _ => idtac
+       end.
+  2: { constructor 1; try refine (@eq_refl bool true).
+       2: { hnf.
+            Print PCUICEquality.eq_term_upto_univ_napp.
+             reflexivity.
+             constructor.
+             reflexivity.
+        cbn.
+       refine (eq_refl true).
+        cbn.
+  2: { match goal with
+  match goal
+  all: match goal with |- _ ;;; _ |- ?e : _ => is_evar e; shelve | _ => idtac end.
+  4: {
+  match goal with
+  all: try apply cumul_Sort.
+  Print cumulSpec0.
+Set Printing All.
+
+  all:
+  21: { cbv [type_of_constructor inductive_mind fst snd cstr_type ind_bodies subst0 inds List.length subst_instance subst_instance_constr].
+  all: lazymatch goal with
+       | [ |- isType _ _ _ ] => econstructor
+       | _ => idtac
+       end.
+    end ].
+  all: cbn.
+  Search isType tApp.
+  47: {
+  all: cbn.
+  53: { cbv [PCUICLookup.declared_minductive_gen].
+  Search isType tRel.
+  cbn -[wf_universe].
+  cbv [subst_instance subst_instance_univ0 NonEmptySetFacts.map].
+  Set Printing All.
+  Search isType tSort.
+  lazymatch goal with
+  end.
+  Search isType tProd.
+  all: repeat first [ progress cbn [type_of_constructor ind_type ind_bodies inductive_ind nth_error]
+                    | eassumption
+                    | reflexivity
+                    | match goal with
+                      | [ |- declared_inductive _ _ _ _ ] => eapply declared_inductive_from_gen; constructor; hnf
+                      | [ |- declared_constructor _ _ _ _ _ ] => eapply declared_constructor_from_gen; repeat apply conj
+                      end ].
+  all: repeat first [ progress cbn [type_of_constructor ind_type ind_bodies inductive_ind nth_error]
+                    | progress cbv [type_of_constructor ind_type]
+                    | eassumption
+                    | reflexivity
+                    | match goal with
+                      | [ |- declared_inductive _ _ _ _ ] => eapply declared_inductive_from_gen; constructor; hnf
+                      | [ |- declared_constructor _ _ _ _ _ ] => eapply declared_constructor_from_gen; repeat apply conj
+                      | [ |- isType _ _ _ ] => eexists
+                      end ].
+  all: cbn.
+  all: repeat first [ reflexivity
+                    | eassumption
+                    | match goal with
+                      | [ |- _;;;_ |- tProd _ _ _ : _ ] => eapply type_Prod
+                      | [ |- _;;;_ |- tSort _ : _ ] => eapply type_Sort
+                      | [ |- _;;;_ |- tRel _ : _ ] => (idtac + eapply type_Cumul); [ eapply type_Rel | .. ]
+                      | [ |- _;;;_ |- tInd _ _ : _ ] => (idtac + eapply type_Cumul); [ eapply type_Ind | .. ]
+                      | [ |- wf_local _ [] ] => constructor
+                      | [ |- wf_local _ [] ] => constructor
+                      | [ |- wf_local _ (_ ,, _) ] => constructor
+                      | [ |- lift_typing _ _ _ _ _ ] => hnf; try eexists
+                      | [ |- declared_inductive _ _ _ _ ] => eapply declared_inductive_from_gen; constructor; hnf
+                      | [ |- declared_constructor _ _ _ _ _ ] => eapply declared_constructor_from_gen; repeat apply conj
+                      end ].
+  all: match goal with |- wf_universe _ _ => shelve | _ => idtac end.
+  all: cbn.
+  cbn.
+  Search wf_universe.
+  2: {  Set Printing All.
+                      | [ |- _;;;_ |- tInd _ _ : _ ] => eapply type_Ind
+                      | [ |- _;;;_ |- tConstruct _ _ _ : _ ] => eapply type_Construct
+Print type_of_constructor.
+  hnf.
+  Print isType.
+  cbn [ind_type].
+  all: lazymatch goal with
+       | _ => idtac
+       end.
+  { constructor.
+    hnf.
+    eassumption.
+  match goal with
+  end.
+  Search declared_inductive lookup_env.
+  Set Printing Implicit.
+  { repeat match goal with
+           end.
+    Search eqb.
+    match goal with
+    end.
+
+  24: {
+  Locate weaken_ctx.
+  Check weaken_ctx.
+  HERE
+  3: { cbn.
+       match goal with
+       end.
+  7: {
+    match goal with
+   end.
+
+  eapply type_Ind.
+  eapply type_mkApps.
+  match goal with
+  end.
+  eapply type_App.
+  2: {
+    match goal with
+    cbn [lift_typing].
+  2: constructor.
+  3: { lazymatch goal with
+    end.
+           (idtac + eapply type_Cumul); [ eapply H | .. ]
+                                         ; eassumption
+
+        constructor 3
+  all: repeat first [ assumption
+                    | match goal with
+                      | [ |- _;;;_ |- tApp _ _ : _ ] => eapply type_App
+                      | [ H : @quotation_of_well_typed _ _ _ _ ?qP  |- _;;;_ |- ?qP : _ ]
+                        => (idtac + eapply type_Cumul); [ eapply H | .. ]
+                      end ].
+  2: {
+  all: repeat first [ assumption
+                    | match goal with
+                      | [ |- _;;;_ |- tApp _ _ : _ ] => eapply type_App
+                      | [ H : @quotation_of_well_typed _ _ _ _ ?qP  |- _;;;_ |- ?qP : _ ]
+                        => (idtac + eapply type_Cumul); [ eapply H | .. ]
+                      end ].
+  2: { match goal with
+                      | [ |- _;;;_ |- tApp _ _ : _ ] => eapply type_App
+                      | [ H : @quotation_of_well_typed _ _ _ _ ?qP  |- _;;;_ |- ?qP : _ ]
+                        => (idtac + eapply type_Cumul); [ eapply H | .. ]
+                      end.
+  eapply type_Prod.
+  3: {
+  all: repeat first [ assumption
+                    | match goal with
+                      | [ |- _;;;_ |- tApp _ _ : _ ] => eapply type_App
+                      | [ |- _;;;_ |- qH : _ ]
+                        => (idtac + eapply type_Cumul); [ eapply qtyH | .. ]
+                      | [ |- _;;;_ |- qP : _ ]
+                        => (idtac + eapply type_Cumul); [ eapply qtyP | .. ]
+                      end ].
+  3: { match goal with
+                 | [ |- _;;;_ |- qP : _ ]
+                   => (idtac + eapply type_Cumul); [ eapply qtyP | .. ]
+    end.
+      eapply qtyP.
+  2: { exactly_once econstructor.
+       Show Proof.
+  2: eapply qtyH.
+         | [ |- _;;;_ |- tProd _ _ _ : _ ] => eapply type_Prod
+  { eapply type_App.
+    eapply type_Prod.
+    3: { eapply qtyH; assumption.
+         assumption.
+         assumption.
+         assumption.
+      hnf in qtyH.
+
+  cbn [mkApps].
+
+  Search typing tApp.
+  Search mkApps typing.
+
+  hnf in qtyH.
+  hnf.
+
+
+Class quotation_of_well_typed {Pcf : config.typing_restriction} {T} (t : T) {qT : quotation_of T} {qt : quotation_of t} := typing_quoted_term_of : forall cf Σ Γ, config.checker_flags_constraint cf -> config.global_env_ext_constraint Σ -> wf_local Σ Γ -> Σ ;;; Γ |- qt : qT.
+Class ground_quotable_well_typed {Pcf : config.typing_restriction} T {qT : quotation_of T} {quoteT : ground_quotable T} := typing_quote_ground : forall t : T, quotation_of_well_typed t.
+
+
+ground_quotable_well_typed {Pcf : config.typing_restriction} T {qT : quotation_of T} {quoteT : ground_quotable T} := typing_quote_ground : forall t : T, quotation_of_well_typed t.
+
+(** Some helper lemmas for defining quotations *)
+Definition ground_quotable_of_bp {b P} (H : b = true -> P) {qH : quotation_of H} (H_for_safety : P -> b = true) : ground_quotable P.
+Proof.
+  intro p.
+  exact (Ast.mkApps qH [_ : quotation_of (@eq_refl bool true)]).
+Defined.
+
+Definition ground_quotable_neg_of_bp {b P} (H : b = false -> ~P) {qH : quotation_of H} (H_for_safety : ~P -> b = false) : ground_quotable (~P).
+Proof.
+  intro p.
+  exact (Ast.mkApps qH [_ : quotation_of (@eq_refl bool false)]).
+Defined.
+
+Definition ground_quotable_of_dec {P} (H : {P} + {~P}) {qP : quotation_of P} {qH : quotation_of H} : ground_quotable P
+  := ground_quotable_of_bp bp_of_dec pb_of_dec.
+Definition ground_quotable_neg_of_dec {P} (H : {P} + {~P}) {qP : quotation_of P} {qH : quotation_of H} : ground_quotable (~P)
+  := ground_quotable_neg_of_bp neg_bp_of_dec neg_pb_of_dec.
+Definition ground_quotable_neq_of_EqDec {A x y} {qA : quotation_of A} {quoteA : ground_quotable A} {H : EqDec A} {qH : quotation_of H} : ground_quotable (x <> y :> A)
+  := ground_quotable_neg_of_dec (H x y).
+#[export] Hint Extern 1 (ground_quotable (?x <> ?y :> ?A)) => simple notypeclasses refine (@ground_quotable_neq_of_EqDec A x y _ _ _ _) : typeclass_instances.
+
+(* avoid universe inconsistencies *)
+#[export] Polymorphic Instance qfst_cps {A B} {qA : quotation_of A} {qB : quotation_of B} : quotation_of (@fst A B) | 0
+  := tApp <% @fst %> [qA; qB].
+#[export] Polymorphic Instance qsnd_cps {A B} {qA : quotation_of A} {qB : quotation_of B} : quotation_of (@snd A B) | 0
+  := tApp <% @snd %> [qA; qB].
+#[export] Polymorphic Instance qpair_cps {A B} {qA : quotation_of A} {qB : quotation_of B} : quotation_of (@pair A B) | 0
+  := tApp <% @pair %> [qA; qB].
+#[export] Polymorphic Instance qprod_cps {A B} {qA : quotation_of A} {qB : quotation_of B} : quotation_of (@prod A B) | 0
+  := tApp <% @prod %> [qA; qB].
+#[export] Polymorphic Instance qSome_cps {A} {qA : quotation_of A} : quotation_of (@Some A) | 0
+  := tApp <% @Some %> [qA].
+#[export] Polymorphic Instance qNone_cps {A} {qA : quotation_of A} : quotation_of (@None A) | 0
+  := tApp <% @None %> [qA].
+#[export] Polymorphic Instance qoption_cps {A} {qA : quotation_of A} : quotation_of (@option A) | 0
+  := tApp <% @option %> [qA].
+#[export] Polymorphic Instance qcons_cps {A} {qA : quotation_of A} : quotation_of (@cons A) | 0
+  := tApp <% @cons %> [qA].
+#[export] Polymorphic Instance qnil_cps {A} {qA : quotation_of A} : quotation_of (@nil A) | 0
+  := tApp <% @nil %> [qA].
+#[export] Polymorphic Instance qlist_cps {A} {qA : quotation_of A} : quotation_of (@list A) | 0
+  := tApp <% @list %> [qA].
+
+Polymorphic Definition ground_quotable_of_iffT {A B} {quoteA : ground_quotable A} {qA : quotation_of A} {qB : quotation_of B} (H : A <~> B) {qH : quotation_of H} : ground_quotable B.
+Proof.
+  intro b.
+  change (@quotation_of B (fst H (snd H b))).
+  make_quotation_of_goal ().
+Defined.
+(* Transparent versions *)
+Definition proj1 {A B} (x : A /\ B) : A := ltac:(apply x).
+Definition proj2 {A B} (x : A /\ B) : B := ltac:(apply x).
+Definition ground_quotable_of_iff {A B : Prop} {quoteA : ground_quotable A} {qA : quotation_of A} {qB : quotation_of B} (H : iff A B) {qH : quotation_of H} : ground_quotable B.
+Proof.
+  intro b.
+  change (@quotation_of B (proj1 H (proj2 H b))).
+  exact _.
+Defined.
+Definition quote_neg_of_iffT {A B} {quoteA : ground_quotable (A -> False)} {qA : quotation_of A} {qB : quotation_of B} (H : A <~> B) {qH : quotation_of H} : ground_quotable (B -> False).
+Proof.
+  intro nb.
+  assert (na : A -> False) by (intro a; apply nb, H, a).
+  change (@quotation_of (B -> False) (fun b => na (snd H b))).
+  exact _.
+Defined.
+Definition quote_neg_of_iff {A B : Prop} {quoteA : ground_quotable (~A)} {qA : quotation_of A} {qB : quotation_of B} (H : iff A B) {qH : quotation_of H} : ground_quotable (~B).
+Proof.
+  intro nb.
+  assert (na : ~A) by (intro a; apply nb, H, a).
+  change (@quotation_of (~B) (fun b => na (proj2 H b))).
+  exact _.
+Defined.
+
+Ltac unfold_quotation_of _ :=
+  lazymatch goal with
+  | [ |- @quotation_of ?A ?t ]
+    => first [ progress cbv delta [t]
+             | change (@quotation_of A (transparentify t)) ]
+  end.
+
+(* for universe adjustment with [tmDeclareQuotationOfModule], [tmMakeQuotationOfModule] *)
+#[export] Unset MetaCoq Strict Unquote Universe Mode.
+(* N.B. We need to kludge around COQBUG(https://github.com/coq/coq/issues/17303) in Kernames :-( *)
+Polymorphic Definition tmMakeQuotationOfConstants_gen@{d t u _T _above_u'} {debug:debug_opt} (work_around_coq_bug_17303 : bool) (include_submodule : list ident -> bool) (include_supermodule : list ident -> list ident -> bool) (existing_instance : option hint_locality) (base : modpath) (cs : list global_reference) (tmDoWithDefinition : ident -> forall A : Type@{d}, A -> TemplateMonad@{t u} A) : TemplateMonad@{t u} unit
+  := let warn_bad_ctx c ctx :=
+       (_ <- tmMsg "tmPrepareMakeQuotationOfModule: cannot handle polymorphism";;
+        _ <- tmPrint c;;
+        _ <- tmPrint ctx;;
+        tmReturn tt) in
+     let tmDebugMsg s := (if debug
+                          then tmMsg s
+                          else tmReturn tt) in
+     let tmDebugPrint {T : Type@{_T}} (v : T)
+       := (if debug
+           then tmPrint v
+           else tmReturn tt) in
+     let on_bad_relevance r :=
+       (_ <- tmDebugMsg "skipping irrelevant constant";;
+        _ <- tmDebugPrint r;;
+        tmReturn tt) in
+     let make_qname '(mp, name)
+       (* ideally we'd replace _ with __ so that there can't be any collision, but the utility functions aren't written and we don't need it in practice *)
+       := option_map
+            (fun n => "q" ++ n)%bs
+            match split_common_prefix base mp with
+            | None => if include_supermodule [] []
+                      then Some name
+                      else None
+            | Some (_, (_common, [], [])) => Some name
+            | Some (_, (_common, [], postfix))
+              => if include_submodule postfix
+                 then Some (String.concat "__DOT__" postfix ++ "__" ++ name)
+                 else None
+            | Some (_, (_common, base_postfix, postfix))
+              => if include_supermodule base_postfix postfix
+                 then Some ("__DOT_DOT__" ++ String.concat "__DOT__" base_postfix ++ "__SLASH__" ++ String.concat "__DOT__" postfix ++ "__" ++ name)
+                 else None
+            end%bs in
+     let tmDebugSkipGR '(mp, name) :=
+       _ <- tmDebugMsg ("tmMakeQuotationOfConstants_gen: skipping excluded constant " ++ name);;
+       _ <- tmDebugPrint (split_common_prefix base mp);;
+       ret tt in
+     let make_definition '(name, tyv)
+       := ((let tmTyv := tmRetypeAroundMetaCoqBug853 name tyv in
+            _ <- tmDebugPrint tmTyv;;
+            '{| my_projT1 := ty ; my_projT2 := v |} <- tmTyv;;
+            tmDef_name <- tmEval cbv (@tmDoWithDefinition (name:string));;
+            let tmn := tmDef_name ty v in
+            _ <- tmDebugPrint tmn;;
+            n <- tmn;;
+            _ <- tmDebugMsg "tmMakeQuotationOfConstants_gen: tmQuoteToGlobalReference";;
+            qn <- tmQuoteToGlobalReference n;;
+            tmReturn qn) : TemplateMonad global_reference) in
+     let make_instance p
+       := (match existing_instance return TemplateMonad unit with
+           | Some locality
+             => let tmEx := tmExistingInstance locality p in
+                _ <- tmDebugPrint tmEx;;
+                tmEx
+           | None => tmReturn tt
+           end) in
+     let cs := dedup_grefs cs in
+     cs <- tmEval cbv cs;;
+     _ <- tmDebugMsg "tmMakeQuotationOfConstants_gen: looking up module constants";;
+     ps <- monad_map@{_ _ Set _above_u'}
+             (fun r
+              => _ <- tmDebugMsg "tmMakeQuotationOfConstants_gen: handling";;
+                 _ <- tmDebugPrint r;;
+                 match r with
+                 | ConstRef cr
+                   => match make_qname cr with
+                      | None => tmDebugSkipGR cr
+                      | Some qname
+                        => '(univs, rel) <- tmQuoteConstantUniversesAndRelevance cr false;;
+                           match rel with
+                           | Irrelevant => on_bad_relevance cr
+                           | Relevant
+                             => inst <- match univs with
+                                        | Monomorphic_ctx => tmReturn ([] : Instance.t)
+                                        | (Polymorphic_ctx (univs, constraints)) as ctx
+                                          => _ <- warn_bad_ctx cr ctx;;
+                                             tmReturn ([] : Instance.t)
+                                        end;;
+                                let c := tConst cr inst in
+                                _ <- tmDebugMsg "tmMakeQuotationOfConstants_gen: tmUnquote";;
+                                '{| my_projT1 := cty ; my_projT2 := cv |} <- tmUnquote c;;
+                                _ <- tmDebugMsg "tmMakeQuotationOfConstants_gen: tmUnquote done";;
+                                def <- make_definition
+                                         (qname, if work_around_coq_bug_17303
+                                                 then {| my_projT1 := term ; my_projT2 := c |}
+                                                 else {| my_projT1 := @quotation_of cty cv ; my_projT2 := c |});;
+                                make_instance def
+                           end
+                      end
+                 | IndRef ind
+                   => let '{| inductive_mind := r |} := ind in
+                      match make_qname r with
+                      | None => tmDebugSkipGR r
+                      | Some qname
+                        => inst <- (univs <- tmQuoteInductiveUniverses r;;
+                                    match univs with
+                                    | Monomorphic_ctx => tmReturn ([] : Instance.t)
+                                    | (Polymorphic_ctx (univs, constraints)) as ctx
+                                      => _ <- warn_bad_ctx r ctx;;
+                                         tmReturn ([] : Instance.t)
+                                    end);;
+                           let c := tInd ind inst in
+                           _ <- tmDebugMsg "tmMakeQuotationOfConstants_gen: tmUnquote";;
+                           '{| my_projT1 := cty ; my_projT2 := cv |} <- tmUnquote c;;
+                           _ <- tmDebugMsg "tmMakeQuotationOfConstants_gen: tmUnquote done";;
+                           let tmcty := tmRetypeRelaxSetInCodomain@{t t u} qname cty in
+                           _ <- tmDebugPrint tmcty;;
+                           cty <- tmcty;;
+                           let tmcv := tmObj_magic (B:=cty) cv in
+                           _ <- tmDebugPrint tmcv;;
+                           cv <- tmcv;;
+                           let ty := @inductive_quotation_of cty cv in
+                           let v : ty := {| qinductive := ind ; qinst := inst |} in
+                           def <- make_definition
+                                    (qname, {| my_projT1 := ty ; my_projT2 := v |});;
+                           make_instance def
+                      end
+                 | ConstructRef _ _ | VarRef _ => tmReturn tt
+                 end)
+             cs;;
+     ret tt.
+
+Definition tmMakeQuotationOfConstants {debug:debug_opt} (include_submodule : list ident -> bool) (include_supermodule : list ident -> list ident -> bool) (existing_instance : option hint_locality) (base : modpath) (cs : list global_reference) : TemplateMonad unit
+  := tmMakeQuotationOfConstants_gen false include_submodule include_supermodule existing_instance base cs (fun name ty body => @tmDefinition name ty body).
+
+Definition tmMakeQuotationOfConstantsWorkAroundCoqBug17303 {debug:debug_opt} (include_submodule : list ident -> bool) (include_supermodule : list ident -> list ident -> bool) (base : modpath) (cs : list global_reference) : TemplateMonad unit
+  := tmMakeQuotationOfConstants_gen true include_submodule include_supermodule None base cs (fun name ty body => @tmDefinition name ty body).
+
+Definition tmDeclareQuotationOfConstants {debug:debug_opt} (include_submodule : list ident -> bool) (include_supermodule : list ident -> list ident -> bool) (existing_instance : option hint_locality) (base : modpath) (cs : list global_reference) : TemplateMonad unit
+  := tmMakeQuotationOfConstants_gen false include_submodule include_supermodule existing_instance base cs (fun name ty _ => @tmAxiom name ty).
+
+Variant submodule_inclusion := only_toplevel | all_submodules_except (_ : list (list ident)) | toplevel_and_submodules (_ : list (list ident)) | everything.
+
+#[local] Typeclasses Transparent ident IdentOT.t.
+Definition is_submodule_of (super : list ident) (sub : list ident) : bool
+  := firstn #|super| sub == super.
+Definition is_supermodule_of (sub : list ident) (super : list ident) : bool
+  := is_submodule_of super sub.
+Definition include_submodule_of_submodule_inclusion (si : submodule_inclusion) : list ident -> bool
+  := match si with
+     | only_toplevel => fun _ => false
+     | all_submodules_except ls => fun i => negb (existsb (is_supermodule_of i) ls)
+     | toplevel_and_submodules ls => fun i => existsb (is_supermodule_of i) ls
+     | everything => fun _ => true
+     end.
+Definition include_supermodule_of_submodule_inclusion (si : submodule_inclusion) : list ident -> list ident -> bool
+  := match si with
+     | everything => fun _ _ => true
+     | _ => fun _ _ => false
+     end.
+
+Definition tmMakeQuotationOfModule {debug:debug_opt} (include_submodule : submodule_inclusion) (existing_instance : option hint_locality) (m : qualid) : TemplateMonad _
+  := cs <- tmQuoteModule m;;
+     base <- tmLocateModule1 m;;
+     let include_supermodule := include_supermodule_of_submodule_inclusion include_submodule in
+     let include_submodule := include_submodule_of_submodule_inclusion include_submodule in
+     tmMakeQuotationOfConstants include_submodule include_supermodule existing_instance base cs.
+Global Arguments tmMakeQuotationOfModule {_%bool} _ _ _%bs.
+
+Definition tmMakeQuotationOfModuleWorkAroundCoqBug17303 {debug:debug_opt} (include_submodule : submodule_inclusion) (m : qualid) : TemplateMonad _
+  := cs <- tmQuoteModule m;;
+     base <- tmLocateModule1 m;;
+     let include_supermodule := include_supermodule_of_submodule_inclusion include_submodule in
+     let include_submodule := include_submodule_of_submodule_inclusion include_submodule in
+     tmMakeQuotationOfConstantsWorkAroundCoqBug17303 include_submodule include_supermodule base cs.
+Global Arguments tmMakeQuotationOfModuleWorkAroundCoqBug17303 {_%bool} _ _%bs.
+
+Definition tmDeclareQuotationOfModule {debug:debug_opt} (include_submodule : submodule_inclusion) (existing_instance : option hint_locality) (m : qualid) : TemplateMonad _
+  := cs <- tmQuoteModule m;;
+     base <- tmLocateModule1 m;;
+     let include_supermodule := include_supermodule_of_submodule_inclusion include_submodule in
+     let include_submodule := include_submodule_of_submodule_inclusion include_submodule in
+     tmDeclareQuotationOfConstants include_submodule include_supermodule existing_instance base cs.
+Global Arguments tmDeclareQuotationOfModule {_%bool} _ _ _%bs.
+
+(*
+Require Import MSetPositive.
+Instance: debug_opt := true.
+MetaCoq Run (tmMakeQuotationOfModule None "Coq.MSets.MSetPositive.PositiveSet"%bs).
+*)
